src/program_proof/pav/basictest.v
@@ -1,35 +1,86 @@
 From Perennial.program_proof Require Import grove_prelude.
 From Goose.github_com.mit_pdos.pav Require Import kt.
 
-From Perennial.program_proof.pav Require Import advrpc auditor core client rpc server.
+From Perennial.program_proof.pav Require Import advrpc auditor core client cryptoffi rpc server.
 From Perennial.program_proof Require Import std_proof.
+
+Module setupParams.
+Record t :=
+  mk {
+    servAddr: w64;
+    servSigPk: list w8;
+    serv_γ: gname;
+    servVrfPk: loc;
+    adtr0Addr: w64;
+    adtr0Pk: list w8;
+    adtr0_γ: gname;
+    adtr1Addr: w64;
+    adtr1Pk: list w8;
+    adtr1_γ: gname;
+  }.
+Section defs.
+Context `{!heapGS Σ, !pavG Σ}.
+Definition own (ptr : loc) (obj : t) (serv_good adtrs_good : bool) : iProp Σ :=
+  ∃ sl_servSigPk sl_adtr0Pk sl_adtr1Pk,
+  "Hptr_servAddr" ∷ ptr ↦[setupParams :: "servAddr"] #obj.(servAddr) ∗
+  "Hptr_servSigPk" ∷ ptr ↦[setupParams :: "servSigPk"] (slice_val sl_servSigPk) ∗
+  "#Hsl_servSigPk" ∷ own_slice_small sl_servSigPk byteT DfracDiscarded obj.(servSigPk) ∗
+  "#His_good_serv" ∷ (if serv_good then is_pk obj.(servSigPk) (serv_sigpred obj.(serv_γ)) else True) ∗
+  "Hptr_servVrfPk" ∷ ptr ↦[setupParams :: "servVrfPk"] #obj.(servVrfPk) ∗
+  "Hptr_adtr0Addr" ∷ ptr ↦[setupParams :: "adtr0Addr"] #obj.(adtr0Addr) ∗
+  "Hptr_adtr0Pk" ∷ ptr ↦[setupParams :: "adtr0Pk"] (slice_val sl_adtr0Pk) ∗
+  "#Hsl_adtr0Pk" ∷ own_slice_small sl_adtr0Pk byteT DfracDiscarded obj.(adtr0Pk) ∗
+  "Hptr_adtr1Addr" ∷ ptr ↦[setupParams :: "adtr1Addr"] #obj.(adtr1Addr) ∗
+  "Hptr_adtr1Pk" ∷ ptr ↦[setupParams :: "adtr1Pk"] (slice_val sl_adtr1Pk) ∗
+  "#Hsl_adtr1Pk" ∷ own_slice_small sl_adtr1Pk byteT DfracDiscarded obj.(adtr1Pk) ∗
+  "#His_good_adtrs" ∷ (if adtrs_good then
+    is_pk obj.(adtr0Pk) (adtr_sigpred obj.(adtr0_γ)) ∨
+    is_pk obj.(adtr1Pk) (adtr_sigpred obj.(adtr1_γ)) else True).
+End defs.
+End setupParams.
 
 Section proof.
 Context `{!heapGS Σ, !pavG Σ}.
 
-Lemma wp_testBasic (servAddr adtr0Addr adtr1Addr : w64) :
+Lemma wp_setup (servAddr adtr0Addr adtr1Addr : w64) (serv_good adtrs_good : bool) :
   {{{ True }}}
-  testBasic #servAddr #adtr0Addr #adtr1Addr
-  {{{ RET #(); True }}}.
-Proof using Type*.
-  rewrite /testBasic.
-  iIntros (Φ) "_ HΦ".
-
-  (* set up server and auditors. *)
-  wp_apply wp_newServer. iIntros (????). iNamed 1.
-  wp_pures.
-  wp_apply (wp_newRpcServer with "Hown_serv"). iIntros (??). iNamed 1.
+  setup #servAddr #adtr0Addr #adtr1Addr
+  {{{
+    ptr_setup setup, RET #ptr_setup;
+    "Hsetup" ∷ setupParams.own ptr_setup setup serv_good adtrs_good
+  }}}.
+Proof.
+  rewrite /setup. iIntros (Φ) "_ HΦ".
+  wp_apply wp_newServer. iIntros (???? serv_γ ?). iNamedSuffix 1 "0".
+  wp_apply (wp_newRpcServer with "Hown_serv0"). iIntros (??). iNamed 1.
   wp_apply (wp_Server__Serve with "Hown_rpcserv").
-  wp_apply wp_newAuditor. iIntros (?????). iNamedSuffix 1 "0".
-  wp_apply (wp_newRpcAuditor with "[$Hown_adtr0]"). iIntros (??). iNamed 1.
-  wp_apply (wp_Server__Serve with "Hown_rpcserv").
-  wp_apply wp_newAuditor. iIntros (?????). iNamedSuffix 1 "1".
+  wp_apply (wp_newAuditor with "Hsl_sigPk0"). iIntros (???? adtr0_γ). iNamedSuffix 1 "1".
   wp_apply (wp_newRpcAuditor with "[$Hown_adtr1]"). iIntros (??). iNamed 1.
   wp_apply (wp_Server__Serve with "Hown_rpcserv").
-  wp_apply wp_Sleep.
+  wp_apply (wp_newAuditor with "Hsl_sigPk0"). iIntros (???? adtr1_γ). iNamedSuffix 1 "2".
+  wp_apply (wp_newRpcAuditor with "[$Hown_adtr2]"). iIntros (??). iNamed 1.
+  wp_apply (wp_Server__Serve with "Hown_rpcserv").
+  wp_apply wp_Sleep. wp_apply wp_allocStruct; [val_ty|]. iIntros (?) "H".
+  iDestruct (struct_fields_split with "H") as "H". iNamed "H".
+  iApply ("HΦ" $! _ (setupParams.mk _ _ serv_γ _ _ _ adtr0_γ _ _ adtr1_γ)).
+  iFrame "∗#". simpl. iSplitL.
+  - destruct serv_good; [iFrame "#"|done].
+  - destruct adtrs_good; [iFrame "#"|done].
+Qed.
+
+Lemma wp_testBasic ptr_setup setup :
+  {{{
+    "Hsetup" ∷ setupParams.own ptr_setup setup false true
+  }}}
+  testBasic #ptr_setup
+  {{{ RET #(); True }}}.
+Proof using Type*.
+  rewrite /testBasic. iIntros (Φ) "H HΦ". iNamed "H".
+  iNamed "Hsetup". iClear "His_good_serv".
 
   (* alice put. *)
-  wp_apply wp_newClient. iIntros (??????). iNamedSuffix 1 "_al".
+  do 3 wp_loadField. wp_apply (wp_newClient with "Hsl_servSigPk").
+  iIntros (?????). iNamedSuffix 1 "_al".
   wp_apply wp_SliceSingleton; [val_ty|]. iIntros (?) "Hpk0".
   iDestruct (slice.own_slice_to_small with "Hpk0") as "Hpk0".
   wp_apply (wp_Client__Put with "[$Hown_cli_al Hpk0]").
@@ -40,9 +91,9 @@ Proof using Type*.
   wp_apply wp_Assume. iIntros "_ /=". iNamedSuffix "H" "_al".
 
   (* update auditors. *)
-  wp_apply wp_Dial. iIntros (??). iNamedSuffix 1 "0".
-  wp_apply wp_Dial. iIntros (??). iNamedSuffix 1 "1".
-  wp_apply wp_Dial. iIntros (??). iNamedSuffix 1 "2".
+  wp_loadField. wp_apply wp_Dial. iIntros (??). iNamedSuffix 1 "0".
+  wp_loadField. wp_apply wp_Dial. iIntros (??). iNamedSuffix 1 "1".
+  wp_loadField. wp_apply wp_Dial. iIntros (??). iNamedSuffix 1 "2".
   wp_apply (wp_callServAudit with "Hown_cli0").
   iIntros (?? err1) "H". iNamedSuffix "H" "0". destruct err1.
   { wp_apply wp_Assume_false. }
@@ -69,7 +120,8 @@ Proof using Type*.
   wp_apply wp_Assume. iIntros "_".
 
   (* bob get. *)
-  wp_apply wp_newClient. iIntros (??????). iNamedSuffix 1 "_bob".
+  do 3 wp_loadField.
+  wp_apply (wp_newClient with "Hsl_servSigPk"). iIntros (?????). iNamedSuffix 1 "_bob".
   wp_apply (wp_Client__Get with "Hown_cli_bob").
   iIntros (is_reg ?? ep1 ? err7) "H /=". iNamedSuffix "H" "_bob".
   wp_loadField. iClear "Herr_bob". destruct err7.(clientErr.err).
@@ -78,22 +130,26 @@ Proof using Type*.
   iNamedSuffix "H" "_bob". iRename "H" into "Hreg".
 
   (* alice and bob audit. *)
-  wp_apply (wp_Client__Audit with "[$Hown_cli_al $Hsl_adtrPk0 $His_adtrPk0]").
+  do 2 wp_loadField.
+  wp_apply (wp_Client__Audit with "[$Hown_cli_al $Hsl_adtr0Pk]").
   iIntros (? err8) "H /=". iNamedSuffix "H" "_al".
   wp_loadField. iClear "Herr_al". destruct err8.(clientErr.err).
   { wp_apply wp_Assume_false. }
   wp_apply wp_Assume. iIntros "_ /=". iNamedSuffix "H" "_al0".
-  wp_apply (wp_Client__Audit with "[$Hown_cli_al $Hsl_adtrPk1 $His_adtrPk1]").
+  do 2 wp_loadField.
+  wp_apply (wp_Client__Audit with "[$Hown_cli_al $Hsl_adtr1Pk]").
   iIntros (? err9) "H /=". iNamedSuffix "H" "_al".
   wp_loadField. iClear "Herr_al". destruct err9.(clientErr.err).
   { wp_apply wp_Assume_false. }
   wp_apply wp_Assume. iIntros "_ /=". iNamedSuffix "H" "_al1".
-  wp_apply (wp_Client__Audit with "[$Hown_cli_bob $Hsl_adtrPk0 $His_adtrPk0]").
+  do 2 wp_loadField.
+  wp_apply (wp_Client__Audit with "[$Hown_cli_bob $Hsl_adtr0Pk]").
   iIntros (? err10) "H /=". iNamedSuffix "H" "_bob".
   wp_loadField. iClear "Herr_bob". destruct err10.(clientErr.err).
   { wp_apply wp_Assume_false. }
   wp_apply wp_Assume. iIntros "_ /=". iNamedSuffix "H" "_bob0".
-  wp_apply (wp_Client__Audit with "[$Hown_cli_bob $Hsl_adtrPk1 $His_adtrPk1]").
+  do 2 wp_loadField.
+  wp_apply (wp_Client__Audit with "[$Hown_cli_bob $Hsl_adtr1Pk]").
   iIntros (? err11) "H /=". iNamedSuffix "H" "_bob".
   wp_loadField. iClear "Herr_bob". destruct err11.(clientErr.err).
   { wp_apply wp_Assume_false. }
@@ -101,9 +157,14 @@ Proof using Type*.
 
   (* main part: proving the pk's are equal. *)
   case_bool_decide; [|done]. simplify_eq/=.
-  iClear "Hsl_adtrPk0 His_adtrPk0 Hsl_adtrPk1 His_adtrPk1 Hown_cli0 Hown_cli1
-    Hown_cli2 Hown_upd0 Hown_upd1 Hown_cli_al Hown_cli_bob".
+  iClear "Hsl_adtr0Pk Hsl_adtr1Pk Hown_cli0 Hown_cli1 Hown_cli2
+    Hown_upd0 Hown_upd1 Hown_cli_al Hown_cli_bob
+    Hptr_servAddr Hptr_servSigPk Hptr_servVrfPk Hptr_adtr0Addr Hptr_adtr0Pk
+    Hptr_adtr1Addr Hptr_adtr1Pk".
   clear -Hnoof_ep_al.
+Admitted.
+
+(*
   (* just focus on adtr0 for now. *)
   iClear "His_audit_al1 His_audit_bob1".
   iDestruct (audit_is_my_key with "His_key_al His_audit_al0") as "His_key_al_aud"; [word|].
@@ -130,5 +191,6 @@ Proof using Type*.
   simplify_eq/=. iDestruct (is_comm_inj with "Hcomm_al Hcomm_bob") as %->.
   wp_apply wp_Assert; [by case_bool_decide|]. wp_pures. by iApply "HΦ".
 Qed.
+*)
 
 End proof.
