src/program_proof/pav/server.v
@@ -1,6 +1,8 @@
 From Perennial.program_proof Require Import grove_prelude.
 From Goose.github_com.mit_pdos.pav Require Import kt.
 
+From Perennial.program_proof.pav Require Import cryptoffi.
+
 Section inv.
 Context `{!heapGS Σ}.
 Definition serv_sigpred (γ : gname) : (list w8 → iProp Σ) :=
@@ -23,8 +25,10 @@ Lemma wp_newServer :
   {{{ True }}}
   newServer #()
   {{{
-    ptr_serv (serv : Server.t) (sigPk vrfPk : loc), RET (#ptr_serv, #sigPk, #vrfPk);
-    "Hown_serv" ∷ Server.own ptr_serv serv
+    ptr_serv (serv : Server.t) sl_sigPk sigPk γ (vrfPk : loc), RET (#ptr_serv, slice_val sl_sigPk, #vrfPk);
+    "Hown_serv" ∷ Server.own ptr_serv serv ∗
+    "#Hsl_sigPk" ∷ own_slice_small sl_sigPk byteT DfracDiscarded sigPk ∗
+    "#His_sigPk" ∷ is_pk sigPk (serv_sigpred γ)
   }}}.
 Proof. Admitted.
 End specs.
